BranchingAssemblyLanguage.thy
@@ -2,32 +2,31 @@ theory BranchingAssemblyLanguage
 imports CPU
 begin
 
-datatype branching_assembly =
+datatype b_assembly =
   ABAssm int
 | CBAssm "register set" computation
-| IBAssm "comparison set" "branching_assembly list" "branching_assembly list"
+| IBAssm "comparison set" "b_assembly list" "b_assembly list"
 | JBAssm code_label
 
-type_synonym branching_assembly_program = "code_label \<rightharpoonup> branching_assembly list"
+type_synonym b_assembly_program = "code_label \<rightharpoonup> b_assembly list"
 
-type_synonym branching_assembly_state = "memory \<times> int option \<times> int \<times> branching_assembly list" 
-  (* \<mu>, a, d, pc *)
+type_synonym b_assembly_state = "memory \<times> int option \<times> int \<times> b_assembly list" 
+  (* \<mu>, a, d, \<pi> *)
 
-fun eval_branching_assembly :: "branching_assembly_program \<Rightarrow> branching_assembly_state \<Rightarrow> 
-    branching_assembly_state option" where
-  "eval_branching_assembly \<Pi> (\<mu>, a, d, []) = None"
-| "eval_branching_assembly \<Pi> (\<mu>, a, d, ABAssm x # \<pi>) = Some (\<mu>, Some x, d, \<pi>)"
-| "eval_branching_assembly \<Pi> (\<mu>, Some a, d, CBAssm dst cmp # \<pi>) = (
+fun eval_b_assembly :: "b_assembly_program \<Rightarrow> b_assembly_state \<Rightarrow> b_assembly_state option" where
+  "eval_b_assembly \<Pi> (\<mu>, a, d, []) = None"
+| "eval_b_assembly \<Pi> (\<mu>, a, d, ABAssm x # \<pi>) = Some (\<mu>, Some x, d, \<pi>)"
+| "eval_b_assembly \<Pi> (\<mu>, Some a, d, CBAssm dst cmp # \<pi>) = (
     let n = compute cmp (\<mu> a) a d
     in Some (
       if M \<in> dst then \<mu>(a := n) else \<mu>, 
       Some (if A \<in> dst then n else a), 
       if D \<in> dst then n else d, 
       \<pi>))"
-| "eval_branching_assembly \<Pi> (\<mu>, None, d, CBAssm dst cmp # \<pi>) = None"
-| "eval_branching_assembly \<Pi> (\<mu>, a, d, IBAssm cmp \<pi>\<^sub>t \<pi>\<^sub>f # \<pi>) = 
+| "eval_b_assembly \<Pi> (\<mu>, None, d, CBAssm dst cmp # \<pi>) = None"
+| "eval_b_assembly \<Pi> (\<mu>, a, d, IBAssm cmp \<pi>\<^sub>t \<pi>\<^sub>f # \<pi>) = 
     Some (\<mu>, a, d, (if should_jump d cmp then \<pi>\<^sub>t else \<pi>\<^sub>f) @ \<pi>)"
-| "eval_branching_assembly \<Pi> (\<mu>, a, d, JBAssm s # \<pi>) = (
+| "eval_b_assembly \<Pi> (\<mu>, a, d, JBAssm s # \<pi>) = (
     case \<Pi> s of 
       Some \<pi>' \<Rightarrow> Some (\<mu>, None, d, \<pi>')
     | None \<Rightarrow> None)"
