LinearAssemblyLanguage.thy
@@ -2,20 +2,20 @@ theory LinearAssemblyLanguage
 imports AssemblyLanguage FiniteMap Iterate
 begin
 
-type_synonym linear_assembly_program = "code_label \<leadsto> assembly list"
+type_synonym l_assembly_program = "code_label \<leadsto> assembly list"
 
-fun eval_linear_assembly :: "linear_assembly_program \<Rightarrow> assembly_state \<Rightarrow> assembly_state option" where
-  "eval_linear_assembly \<Pi> (\<mu>, a, d, []) = None"
-| "eval_linear_assembly \<Pi> (\<mu>, a, d, AAssm x # \<pi>) = Some (\<mu>, Some x, d, \<pi>)"
-| "eval_linear_assembly \<Pi> (\<mu>, Some a, d, CAssm dst cmp # \<pi>) = (
+fun eval_l_assembly :: "l_assembly_program \<Rightarrow> assembly_state \<Rightarrow> assembly_state option" where
+  "eval_l_assembly \<Pi> (\<mu>, a, d, []) = None"
+| "eval_l_assembly \<Pi> (\<mu>, a, d, AAssm x # \<pi>) = Some (\<mu>, Some x, d, \<pi>)"
+| "eval_l_assembly \<Pi> (\<mu>, Some a, d, CAssm dst cmp # \<pi>) = (
     let n = compute cmp (\<mu> a) a d
     in Some (
       if M \<in> dst then \<mu>(a := n) else \<mu>, 
       Some (if A \<in> dst then n else a), 
       if D \<in> dst then n else d, 
       \<pi>))"
-| "eval_linear_assembly \<Pi> (\<mu>, None, d, CAssm dst cmp # \<pi>) = None"
-| "eval_linear_assembly \<Pi> (\<mu>, a, d, JAssm jmp s # \<pi>) = (
+| "eval_l_assembly \<Pi> (\<mu>, None, d, CAssm dst cmp # \<pi>) = None"
+| "eval_l_assembly \<Pi> (\<mu>, a, d, JAssm jmp s # \<pi>) = (
     if should_jump d jmp
     then case lookup \<Pi> s of 
         Some \<pi>' \<Rightarrow> Some (\<mu>, None, d, \<pi>')
@@ -25,7 +25,7 @@ fun eval_linear_assembly :: "linear_assembly_program \<Rightarrow> assembly_stat
 (* linearization correct *)
 
 lemma [simp]: "finite (dom \<Pi>) \<Longrightarrow> eval_assembly \<Pi> \<Sigma> = Some \<Sigma>' \<Longrightarrow> 
-    eval_linear_assembly (linearize \<Pi>) \<Sigma> = Some \<Sigma>'"
+    eval_l_assembly (linearize \<Pi>) \<Sigma> = Some \<Sigma>'"
   proof (induction \<Pi> \<Sigma> rule: eval_assembly.induct)
   case 1
     from 1(2) show ?case by simp
@@ -40,7 +40,7 @@ lemma [simp]: "finite (dom \<Pi>) \<Longrightarrow> eval_assembly \<Pi> \<Sigma>
   qed 
 
 theorem linearization_correct [simp]: "iterate (eval_assembly \<Pi>) \<Sigma> \<Sigma>' \<Longrightarrow> finite (dom \<Pi>) \<Longrightarrow> 
-    iterate (eval_linear_assembly (linearize \<Pi>)) \<Sigma> \<Sigma>'"
+    iterate (eval_l_assembly (linearize \<Pi>)) \<Sigma> \<Sigma>'"
   by (induction "eval_assembly \<Pi>" \<Sigma> \<Sigma>' rule: iterate.induct) simp_all
 
 end
