TotalCorrectness.thy
@@ -3,40 +3,50 @@ imports AssemblyToMachine Debranching StackToAssembly
 begin
 
 definition state_convert :: "stack_program \<Rightarrow> stack_state \<Rightarrow> machine_state set" where
-  "state_convert \<Pi> \<Sigma>\<^sub>S = {\<Sigma>\<^sub>M | \<Sigma>\<^sub>A \<Sigma>\<^sub>M. 
-    \<Sigma>\<^sub>A \<in> StackToAssembly.state_convert \<Sigma>\<^sub>S \<and> 
-      \<Sigma>\<^sub>M \<in> AssemblyToMachine.state_convert (linearize (StackToAssembly.program_convert \<Pi>)) \<Sigma>\<^sub>A}"
+  "state_convert \<Pi> \<Sigma>\<^sub>S = {\<Sigma>\<^sub>M | \<Sigma>\<^sub>B \<Sigma>\<^sub>M. 
+    \<Sigma>\<^sub>B \<in> StackToAssembly.state_convert \<Sigma>\<^sub>S \<and> 
+      \<Sigma>\<^sub>M \<in> AssemblyToMachine.state_convert 
+        (linearize (debranch (StackToAssembly.program_convert \<Pi>))) 
+          (Debranching.state_convert (dom (StackToAssembly.program_convert \<Pi>)) \<Sigma>\<^sub>B)}"
 
 definition program_convert :: "stack_program \<Rightarrow> machine_program" where
   "program_convert \<Pi> =
-    AssemblyToMachine.program_convert (linearize (StackToAssembly.program_convert \<Pi>))"
+    AssemblyToMachine.program_convert (linearize (debranch (StackToAssembly.program_convert \<Pi>)))"
 
 theorem total_correctness: "finite (dom \<Pi>) \<Longrightarrow> iterate (eval_stack \<Pi>) \<Sigma>\<^sub>S \<Sigma>\<^sub>S' \<Longrightarrow> 
   \<Sigma>\<^sub>M \<in> state_convert \<Pi> \<Sigma>\<^sub>S \<Longrightarrow> 
     \<exists>\<Sigma>\<^sub>M'. \<Sigma>\<^sub>M' \<in> state_convert \<Pi> \<Sigma>\<^sub>S' \<and> iterate (eval_machine (program_convert \<Pi>)) \<Sigma>\<^sub>M \<Sigma>\<^sub>M'"
   proof -
     assume D: "finite (dom \<Pi>)"
-    hence DL: "domain_distinct (linearize (StackToAssembly.program_convert \<Pi>))" by simp
-    from D have DF: "finite (dom (StackToAssembly.program_convert \<Pi>))" by simp
+    hence DL: "domain_distinct (linearize (debranch (StackToAssembly.program_convert \<Pi>)))" by simp
+    from D have DF: "finite (dom (debranch (StackToAssembly.program_convert \<Pi>)))" by simp
     assume ES: "iterate (eval_stack \<Pi>) \<Sigma>\<^sub>S \<Sigma>\<^sub>S'"
     assume "\<Sigma>\<^sub>M \<in> state_convert \<Pi> \<Sigma>\<^sub>S"
-    with state_convert_def obtain \<Sigma>\<^sub>A where SA: "\<Sigma>\<^sub>A \<in> StackToAssembly.state_convert \<Sigma>\<^sub>S \<and> 
-        \<Sigma>\<^sub>M \<in> AssemblyToMachine.state_convert (linearize (StackToAssembly.program_convert \<Pi>)) \<Sigma>\<^sub>A" 
+    with state_convert_def obtain \<Sigma>\<^sub>B where SA: "\<Sigma>\<^sub>B \<in> StackToAssembly.state_convert \<Sigma>\<^sub>S \<and> 
+        \<Sigma>\<^sub>M \<in> AssemblyToMachine.state_convert 
+          (linearize (debranch (StackToAssembly.program_convert \<Pi>))) 
+            (Debranching.state_convert (dom (StackToAssembly.program_convert \<Pi>)) \<Sigma>\<^sub>B)" 
       by blast
-    with ES stack_to_assembly_correct obtain \<Sigma>\<^sub>A' where SA': 
-      "\<Sigma>\<^sub>A' \<in> StackToAssembly.state_convert \<Sigma>\<^sub>S' \<and> 
-        iterate (eval_assembly (StackToAssembly.program_convert \<Pi>)) \<Sigma>\<^sub>A \<Sigma>\<^sub>A'" by blast
-    with ES DF linearization_correct have 
-      "iterate (eval_linear_assembly (linearize (StackToAssembly.program_convert \<Pi>))) \<Sigma>\<^sub>A \<Sigma>\<^sub>A'" 
-      by blast
+    with ES stack_to_assembly_correct obtain \<Sigma>\<^sub>B' where SA': 
+      "\<Sigma>\<^sub>B' \<in> StackToAssembly.state_convert \<Sigma>\<^sub>S' \<and> 
+        iterate (eval_b_assembly (StackToAssembly.program_convert \<Pi>)) \<Sigma>\<^sub>B \<Sigma>\<^sub>B'" by blast
+    let ?\<Sigma>\<^sub>A = "Debranching.state_convert (dom (StackToAssembly.program_convert \<Pi>)) \<Sigma>\<^sub>B"
+    let ?\<Sigma>\<^sub>A' = "Debranching.state_convert (dom (StackToAssembly.program_convert \<Pi>)) \<Sigma>\<^sub>B'"
+    from SA' ES debranching_correct have 
+      "iterate (eval_assembly (debranch (StackToAssembly.program_convert \<Pi>))) ?\<Sigma>\<^sub>A ?\<Sigma>\<^sub>A'" by blast
+    with DF linearization_correct have 
+      "iterate (eval_l_assembly (linearize (debranch (StackToAssembly.program_convert \<Pi>)))) 
+        ?\<Sigma>\<^sub>A ?\<Sigma>\<^sub>A'" by blast
     with SA DL assembly_to_machine_correct obtain \<Sigma>\<^sub>M' where SM': 
-      "\<Sigma>\<^sub>M' \<in> AssemblyToMachine.state_convert (linearize (StackToAssembly.program_convert \<Pi>)) \<Sigma>\<^sub>A' \<and> 
-        iterate (eval_machine (AssemblyToMachine.program_convert 
-          (linearize (StackToAssembly.program_convert \<Pi>)))) \<Sigma>\<^sub>M \<Sigma>\<^sub>M'" by blast
-    with SA' have "\<Sigma>\<^sub>M' \<in> {\<Sigma>\<^sub>M' | \<Sigma>\<^sub>A' \<Sigma>\<^sub>M'. 
-      \<Sigma>\<^sub>A' \<in> StackToAssembly.state_convert \<Sigma>\<^sub>S' \<and> 
-        \<Sigma>\<^sub>M' \<in> AssemblyToMachine.state_convert (linearize (StackToAssembly.program_convert \<Pi>)) \<Sigma>\<^sub>A'}" 
-      by blast
+      "\<Sigma>\<^sub>M' \<in> AssemblyToMachine.state_convert 
+        (linearize (debranch (StackToAssembly.program_convert \<Pi>))) ?\<Sigma>\<^sub>A' \<and> 
+          iterate (eval_machine (AssemblyToMachine.program_convert 
+            (linearize (debranch (StackToAssembly.program_convert \<Pi>))))) \<Sigma>\<^sub>M \<Sigma>\<^sub>M'" by blast
+    with SA' have "\<Sigma>\<^sub>M' \<in> {\<Sigma>\<^sub>M' | \<Sigma>\<^sub>B' \<Sigma>\<^sub>M'. 
+      \<Sigma>\<^sub>B' \<in> StackToAssembly.state_convert \<Sigma>\<^sub>S' \<and> 
+        \<Sigma>\<^sub>M' \<in> AssemblyToMachine.state_convert 
+          (linearize (debranch (StackToAssembly.program_convert \<Pi>)))  
+            (Debranching.state_convert (dom (StackToAssembly.program_convert \<Pi>)) \<Sigma>\<^sub>B')}" by blast
     with SM' have "\<Sigma>\<^sub>M' \<in> state_convert \<Pi> \<Sigma>\<^sub>S' \<and> iterate (eval_machine (program_convert \<Pi>)) \<Sigma>\<^sub>M \<Sigma>\<^sub>M'"
       by (simp add: state_convert_def program_convert_def)
     thus ?thesis by fastforce
